FunctionApp: try to untangle explicit stack from runStackProcess obligation
Signed-off-by: Anders Kaseorg <andersk@mit.edu>

FunctionApp.v
@@ -6,6 +6,7 @@ Section process.
   | Step : (input -> (world -> world) * process) -> process.
 
   Definition action := world -> world.
+  Definition step := input -> action * process.
 
   Definition runStep wp i :=
     match wp with
@@ -14,6 +15,7 @@ Section process.
 End process.
 
 Arguments process : clear implicits.
+Arguments step : clear implicits.
 Arguments action : clear implicits.
 
 
@@ -24,48 +26,110 @@ Section stackProcess.
   Context {world : Type}.
 
   Definition stackWorld := (list message * action world)%type.
-  Definition stackProcess := process (message + input) stackWorld.
+  Definition stackInput := (message + input)%type.
+  Definition stackProcess := process stackInput stackWorld.
+  Definition stackStep := step stackInput stackWorld.
 
   Definition stackPush (m : message) : action stackWorld :=
     fun sw => let (ms, a) := sw in ((m :: ms)%list, a).
   Definition stackLift (a : action world) : action stackWorld :=
     fun sw => let (ms, a') := sw in (ms, fun w => a (a' w)).
 
-  Inductive emptiesStack :
-    stackWorld * stackProcess -> Prop :=
-  | stackEmpty p :
-      emptiesStack (nil, @id world, p)
-  | popsStack m ms a p :
-      emptiesStack (runStep (ms, a, p) (inl m)) ->
-      emptiesStack ((m :: ms)%list, a, p).
+  Definition stackTransition (m : stackInput) (pf : stackStep) :=
+    (fst (fst (pf m) (nil, @id world)), snd (pf m)).
 
-  Fixpoint stepStackProcess swp (h : emptiesStack swp) : action world * stackProcess.
-  destruct swp as [[[ | m ms] a] p].
-  { exact (a, p). }
+  Inductive emptiesStack : list message * stackProcess -> stackProcess -> Prop :=
+  | stackEmpty p : emptiesStack (nil, p) p
+  | popsStack (m : message) (ms : list message) (pf : stackStep) (p2 p3 : stackProcess) :
+      emptiesStack (stackTransition (inl m) pf) p2 ->
+      emptiesStack (ms, p2) p3 ->
+      emptiesStack ((m :: ms)%list, Step pf) p3.
+
+  CoInductive emptiesStackForever : stackProcess -> Prop :=
+  | emptiesStackStep pf p' :
+      (forall (i : input),
+         emptiesStack (stackTransition (inr i) pf) (p' i) /\
+         emptiesStackForever (p' i)) ->
+      emptiesStackForever (Step pf).
+
+  Inductive stepStackProcessTerminates : list message * stackProcess -> Prop :=
+  | stepStackProcessDone p : stepStackProcessTerminates (nil, p)
+  | stepStackProcessStep m ms pf p2 :
+      stepStackProcessTerminates (stackTransition (inl m) pf) ->
+      emptiesStack (stackTransition (inl m) pf) p2 ->
+      stepStackProcessTerminates (ms, p2) ->
+      stepStackProcessTerminates ((m :: ms)%list, Step pf).
+
+  Fixpoint mkStepStackProcessTerminates mp p' (e : emptiesStack mp p') : stepStackProcessTerminates mp.
+  destruct e; econstructor; eauto.
+  Defined.
+
+  Fixpoint stepStackProcess mp (h : stepStackProcessTerminates mp) :
+    action world * sig (unique (emptiesStack mp)).
+  destruct mp as [[| m ms] p].
   {
-    refine (stepStackProcess (runStep (ms, a, p) (inl m)) _).
-    inversion h; trivial.
+    split.
+    { exact (@id world). }
+    {
+      exists p.
+      split.
+      { constructor. }
+      {
+        inversion 1.
+        reflexivity.
+      }
+    }
+  }
+  {
+    destruct p as [pf].
+    pose (sap1 := pf (inl m)).
+    pose (sw := fst sap1 (nil, @id world)).
+    assert (stepStackProcessTerminates (fst sw, snd sap1)) as e1 by (inversion h; assumption).
+    destruct (stepStackProcess (fst sw, snd sap1) e1) as [a2 [p2 [e2 u2]]].
+    assert (stepStackProcessTerminates (ms, p2)) as e3.
+    {
+      inversion h as [| ? ? ? p'].
+      rewrite (u2 p'); assumption.
+    }
+    destruct (stepStackProcess (ms, p2) e3) as [a3 [p3 [e4 u4]]].
+    split.
+    { exact (fun w => a3 (a2 (snd sw w))). }
+    {
+      exists p3.
+      split.
+      { econstructor; eassumption. }
+      {
+        intros p3' e5.
+        apply u4.
+        inversion e5 as [| ? ? ? p'].
+        rewrite (u2 p'); assumption.
+      }
+    }
   }
   Defined.
 
-  CoInductive emptiesStackForever : stackProcess -> Prop :=
-  | emptiesStackStep p h :
-      (forall (i : input),
-         emptiesStackForever (snd (stepStackProcess
-                                     (runStep (nil, @id world, p) (inr i)) (h i)))) ->
-      emptiesStackForever p.
-
   CoFixpoint runStackProcess (p : stackProcess) (h : emptiesStackForever p) : process input world.
-  refine
-    (Step (fun i =>
-             let ap' :=
-                 stepStackProcess
-                   (runStep (nil, @id world, p) (inr i))
-                   match h with
-                     | emptiesStackStep _ h1 _ => h1 i
-                   end in
-             (fst ap', runStackProcess (snd ap') _))).
-  destruct h; eauto.
+  constructor.
+  intro i.
+  destruct p as [pf].
+  pose (sap1 := pf (inr i)).
+  pose (sw := fst sap1 (nil, @id world)).
+  assert (stepStackProcessTerminates (fst sw, snd sap1)) as e1.
+  {
+    inversion h as [? ? h1].
+    destruct (h1 i).
+    eapply mkStepStackProcessTerminates.
+    eassumption.
+  }
+  destruct (stepStackProcess (fst sw, snd sap1) e1) as [a2 [p2 [e2 u2]]].
+  split.
+  { exact (fun w => a2 (snd sw w)). }
+  {
+    apply (runStackProcess p2).
+    inversion h as [? ? h1].
+    destruct (h1 i).
+    rewrite (u2 (p' i)); assumption.
+  }
   Defined.
 
 End stackProcess.
